Move (action-)events out of reactor, into execution state

src/ReactorModel/Execution/Reactor.lean
@@ -1,29 +1,6 @@
 import ReactorModel.Execution.Dependency
 import Mathlib.Data.Finset.Lattice
 
-namespace List
-
-def targets (cs : List Change) :=
-  { t : Component.Valued × ID | ∃ c ∈ cs, c.Targets t.fst t.snd }
-
-theorem mem_targets_cons (h : t ∈ tl.targets) : t ∈ (hd :: tl).targets := by
-  have ⟨c, hm, _⟩ := h 
-  exists c, by simp [hm]
-
-theorem target_mem_targets {cs : List Change} (hc : c ∈ cs) (ht : c.target = some t) : 
-    t ∈ cs.targets := by
-  exists c, hc
-  cases c <;> simp [Change.target] at *
-  subst ht
-  constructor
-
-end List
-
-def Action.schedule (a : Action) (t : Time) (v : Value) : Action :=
-  match a.tags.filter (·.time = t) |>.max with
-  | ⊥           => a.insert ⟨t, 0⟩ v
-  | some ⟨_, m⟩ => a.insert ⟨t, m + 1⟩ v
-
 -- TODO: Split up the following definitions into appropriate namespaces.
 namespace ReactorType
 namespace Practical
@@ -48,16 +25,6 @@ theorem Cleared.deterministic {rtr : α} (cl₁ : Cleared rtr rtr₁) (cl₂ : C
   case inp => simp_all [(ho₁ ▸ cl₁.inputs)   ▸ (ho₂ ▸ cl₂.inputs)] 
   case out => simp_all [(ho₁ ▸ cl₁.outputs)  ▸ (ho₂ ▸ cl₂.outputs)] 
 
-def apply (rtr : α) : Change → α 
-  | .inp i v   => Updatable.update rtr .inp i (fun _ => v)
-  | .out i v   => Updatable.update rtr .out i (fun _ => v)
-  | .stv i v   => Updatable.update rtr .stv i (fun _ => v)
-  | .act i t v => Updatable.update rtr .act i (·.schedule t v)
-  | .mut ..    => rtr -- Mutations are currently no-ops.
-
-def apply' (rtr : α) (cs : List Change) : α :=
-  cs.foldl apply rtr
-
 def dependencies (rtr : α) (rcn : ID) : Set ID := 
   { rcn' | rcn' <[rtr] rcn }
 
@@ -78,89 +45,5 @@ theorem mem_dependencies_ssubset {rtr : α} {rcn₁ rcn₂ : ID}
     dependencies rtr rcn₂ ⊂ dependencies rtr rcn₁ :=
   ssubset_iff_subset_ne.mpr ⟨mem_dependencies_subset h, (a _ $ ·.symm ▸ h)⟩
 
-def scheduledTags (rtr : α) : Set Time.Tag := 
-  { g | ∃ i a, (rtr[.act][i] = some a) ∧ (g ∈ a.keys) }
-
-scoped macro "cases_change " change:term : tactic => `(tactic| 
-  cases $change:term <;> try cases ‹Change.Normal›; cases ‹Component.Valued›
-)
-
-theorem apply_equiv (rtr : α) (c : Change) : (apply rtr c) ≈ rtr := by
-  cases_change c <;> first | exact .refl _ | apply Equivalent.symm; apply LawfulUpdatable.equiv
-
-theorem apply_preserves_unchanged {c : Change} (rtr : α) (h : ¬c.Targets cpt i) :
-    (apply rtr c)[cpt][i] = rtr[cpt][i] := by
-  cases_change c
-  all_goals first | exact .refl _ | exact LawfulUpdatable.obj?_preserved (Change.Targets.norm_not h)
-
-variable {rtr : α}
-
-theorem apply_input_change (h : i ∈ rtr[.inp]) : (apply rtr $ .inp i v)[.inp][i] = some v := by
-  simp [apply, LawfulUpdatable.obj?_updated]
-  exact h
-
-theorem apply_output_change (h : i ∈ rtr[.out]) : (apply rtr $ .out i v)[.out][i] = some v := by
-  simp [apply, LawfulUpdatable.obj?_updated]
-  exact h
-
-theorem apply_state_change (h : i ∈ rtr[.stv]) : (apply rtr $ .stv i v)[.stv][i] = some v := by
-  simp [apply, LawfulUpdatable.obj?_updated]
-  exact h
-
-theorem apply_action_change (h : rtr[.act][i] = some a) : 
-    (apply rtr $ .act i t v)[.act][i] = some (a.schedule t v) := by
-  simp [apply, LawfulUpdatable.obj?_updated]
-  exact ⟨_, ⟨h, rfl⟩⟩ 
-
-theorem apply_ne_target_comm (ht : c₁.target ≠ c₂.target ∨ c₁.target = none) : 
-    apply (apply rtr c₁) c₂ = apply (apply rtr c₂) c₁ := by
-  cases_change c₁ <;> cases_change c₂ <;> simp [apply, Change.target] at *
-  all_goals exact LawfulUpdatable.update_ne_comm $ by simp_all
-    
-theorem apply'_equiv (rtr : α) : (cs : List Change) → (apply' rtr cs) ≈ rtr 
-  | .nil        => .refl _
-  | .cons hd tl => Equivalent.trans (apply'_equiv (apply rtr hd) tl) (apply_equiv rtr hd)
-
-theorem apply'_preserves_unchanged {cs : List Change} {cpt : Component.Valued} {i}
-    (h : cs.All₂ (¬·.Targets cpt i)) : (apply' rtr cs)[cpt][i] = rtr[cpt][i] := by
-  induction cs generalizing rtr <;> try rfl
-  case cons hd tl hi => 
-    have ⟨hh, ht⟩ := List.all₂_cons _ _ _ |>.mp h
-    exact apply_preserves_unchanged rtr hh ▸ hi ht 
-
-theorem apply'_apply_ne_targets_comm (ht : ∀ {t}, c.target = some t → t ∉ cs.targets) : 
-    apply (apply' rtr cs) c = apply' (apply rtr c) cs := by
-  induction cs generalizing rtr <;> simp [apply'] at *
-  case cons hd tl hi =>
-    suffices h : hd.target ≠ c.target ∨ hd.target = none by 
-      rw [hi $ fun _ _ h hm => ht _ _ h $ List.mem_targets_cons hm, apply_ne_target_comm h]
-    by_contra hc
-    push_neg at hc
-    have ⟨_, h⟩ := Option.ne_none_iff_exists.mp hc.right
-    exact ht _ _ (hc.left ▸ h.symm) $ List.target_mem_targets (by simp) h.symm
-
-theorem apply'_disjoint_targets_comm (ht : Disjoint cs₁.targets cs₂.targets) : 
-    apply' (apply' rtr cs₁) cs₂ = apply' (apply' rtr cs₂) cs₁ := by
-  induction cs₁ generalizing rtr <;> cases cs₂ <;> simp [apply'] at *
-  case cons.cons hd₁ tl₁ hd₂ tl₂ hi =>
-    have h₁ : Disjoint (List.targets tl₁) (List.targets (hd₂ :: tl₂)) := by
-      simp [Set.disjoint_iff_forall_ne]
-      intro _ _ hm₁ _ _ hm₂ h₁ h₂
-      subst h₁ h₂    
-      exact Set.disjoint_left.mp ht (List.mem_targets_cons hm₁) hm₂
-    have h₂ : hd₁.target ≠ hd₂.target ∨ hd₁.target = none := by
-      by_contra hc
-      push_neg at hc
-      have ⟨_, h⟩ := Option.ne_none_iff_exists.mp hc.right
-      have h₁ := (hd₁ :: tl₁).target_mem_targets (by simp) h.symm
-      have h₂ := (hd₂ :: tl₂).target_mem_targets (by simp) (hc.left ▸ h.symm)
-      exact Set.disjoint_left.mp ht h₁ h₂
-    have h₃ : ∀ {t}, hd₁.target = some t → ¬t ∈ tl₂.targets := by
-      intro _ h hm
-      have h₁ := (hd₁ :: tl₁).target_mem_targets (by simp) h
-      exact Set.disjoint_left.mp ht h₁ $ List.mem_targets_cons hm
-    rw [hi h₁, apply_ne_target_comm h₂, ←apply', ←apply', ←apply'_apply_ne_targets_comm h₃]
-    rfl
-    
 end Practical
 end ReactorType
