src/ReactorModel/Execution/State.lean
@@ -3,17 +3,143 @@ import ReactorModel.Execution.Reactor
 noncomputable section
 open Classical ReactorType Practical
 
+namespace List
+
+def targets (cs : List Change) :=
+  { t : Component.Valued × ID | ∃ c ∈ cs, c.Targets t.fst t.snd }
+
+theorem mem_targets_cons (h : t ∈ tl.targets) : t ∈ (hd :: tl).targets := by
+  have ⟨c, hm, _⟩ := h 
+  exists c, by simp [hm]
+
+theorem target_mem_targets {cs : List Change} (hc : c ∈ cs) (ht : c.target = some t) : 
+    t ∈ cs.targets := by
+  exists c, hc
+  cases c <;> simp [Change.target] at *
+  subst ht
+  constructor
+
+end List
+
 namespace Execution
 
+infix:50 " ⇉ " => (Finmap fun _ : · => ·)
+
+-- TODO?: Factor out a context again.
 @[ext]
 structure State (α) [Practical α] where
-  rtr : α 
-  tag : Time.Tag
+  rtr      : α 
+  tag      : Time.Tag
   progress : Set ID
+  events   : ID ⇀ Time.Tag ⇉ Value -- For each action we keep a mapping of tag to value.
 
 variable [Practical α]
 
 namespace State
+
+def schedule (a : Time.Tag ⇉ Value) (t : Time) (v : Value) : Time.Tag ⇉ Value :=
+  match a.keys.filter (·.time = t) |>.max with
+  | ⊥           => a.insert ⟨t, 0⟩ v
+  | some ⟨_, m⟩ => a.insert ⟨t, m + 1⟩ v
+
+def apply (s : State α) : Change → State α 
+  | .inp i v   => { s with    rtr := Updatable.update s.rtr .inp i v }
+  | .out i v   => { s with    rtr := Updatable.update s.rtr .out i v }
+  | .stv i v   => { s with    rtr := Updatable.update s.rtr .stv i v }
+  | .act i t v => { s with events := s.events.update i (schedule · t v) }
+  | .mut ..    => s -- Mutations are currently no-ops.
+
+def apply' (s : State α) (cs : List Change) : State α :=
+  cs.foldl apply s
+
+def scheduledTags (s : State α) : Set Time.Tag := 
+  { g | ∃ i a, (s.events i = some a) ∧ (g ∈ a.keys) }
+
+scoped macro "cases_change " change:term : tactic => `(tactic| 
+  cases $change:term <;> try cases ‹Change.Normal›; cases ‹Component.Valued›
+)
+
+theorem apply_equiv (s : State α) (c : Change) : (apply s c).rtr ≈ s.rtr := by
+  cases_change c <;> first | exact .refl _ | apply Equivalent.symm; apply LawfulUpdatable.equiv
+
+theorem apply_preserves_unchanged {c : Change} (s : State α) (h : ¬c.Targets cpt i) :
+    (apply s c).rtr[cpt][i] = s.rtr[cpt][i] := by
+  cases_change c
+  all_goals first | exact .refl _ | exact LawfulUpdatable.obj?_preserved (Change.Targets.norm_not h)
+
+variable {s : State α} in section
+
+theorem apply_input_change (h : i ∈ s.rtr[.inp]) : (apply s $ .inp i v).rtr[.inp][i] = some v := by
+  simp [apply, LawfulUpdatable.obj?_updated]
+  exact h
+
+theorem apply_output_change (h : i ∈ s.rtr[.out]) : (apply s $ .out i v).rtr[.out][i] = some v := by
+  simp [apply, LawfulUpdatable.obj?_updated]
+  exact h
+
+theorem apply_state_change (h : i ∈ s.rtr[.stv]) : (apply s $ .stv i v).rtr[.stv][i] = some v := by
+  simp [apply, LawfulUpdatable.obj?_updated]
+  exact h
+
+theorem apply_ne_target_comm (ht : c₁.target ≠ c₂.target ∨ c₁.target = none) : 
+    apply (apply s c₁) c₂ = apply (apply s c₂) c₁ := by
+  sorry -- by ext1?
+  /-cases_change c₁ <;> cases_change c₂ <;> simp [apply, Change.target] at *
+  all_goals exact LawfulUpdatable.update_ne_comm $ by simp_all
+  -/  
+
+theorem apply'_equiv (s : State α) : (cs : List Change) → (apply' s cs).rtr ≈ s.rtr 
+  | .nil        => .refl _
+  | .cons hd tl => Equivalent.trans (apply'_equiv (apply s hd) tl) (apply_equiv s hd)
+
+theorem apply'_preserves_tag {cs : List Change} : (apply' s cs).tag = s.tag := by
+  sorry
+
+theorem apply'_preserves_progress {cs : List Change} : (apply' s cs).progress = s.progress := by
+  sorry
+
+theorem apply'_preserves_unchanged {cs : List Change} {cpt : Component.Valued} {i}
+    (h : cs.All₂ (¬·.Targets cpt i)) : (apply' s cs).rtr[cpt][i] = s.rtr[cpt][i] := by
+  induction cs generalizing s <;> try rfl
+  case cons hd tl hi => 
+    have ⟨hh, ht⟩ := List.all₂_cons _ _ _ |>.mp h
+    exact apply_preserves_unchanged s hh ▸ hi ht 
+
+theorem apply'_apply_ne_targets_comm (ht : ∀ {t}, c.target = some t → t ∉ cs.targets) : 
+    apply (apply' s cs) c = apply' (apply s c) cs := by
+  induction cs generalizing s <;> simp [apply'] at *
+  case cons hd tl hi =>
+    suffices h : hd.target ≠ c.target ∨ hd.target = none by 
+      rw [hi $ fun _ _ h hm => ht _ _ h $ List.mem_targets_cons hm, apply_ne_target_comm h]
+    by_contra hc
+    push_neg at hc
+    have ⟨_, h⟩ := Option.ne_none_iff_exists.mp hc.right
+    exact ht _ _ (hc.left ▸ h.symm) $ List.target_mem_targets (by simp) h.symm
+
+theorem apply'_disjoint_targets_comm (ht : Disjoint cs₁.targets cs₂.targets) : 
+    apply' (apply' s cs₁) cs₂ = apply' (apply' s cs₂) cs₁ := by
+  induction cs₁ generalizing s <;> cases cs₂ <;> simp [apply'] at *
+  case cons.cons hd₁ tl₁ hd₂ tl₂ hi =>
+    have h₁ : Disjoint (List.targets tl₁) (List.targets (hd₂ :: tl₂)) := by
+      simp [Set.disjoint_iff_forall_ne]
+      intro _ _ hm₁ _ _ hm₂ h₁ h₂
+      subst h₁ h₂    
+      exact Set.disjoint_left.mp ht (List.mem_targets_cons hm₁) hm₂
+    have h₂ : hd₁.target ≠ hd₂.target ∨ hd₁.target = none := by
+      by_contra hc
+      push_neg at hc
+      have ⟨_, h⟩ := Option.ne_none_iff_exists.mp hc.right
+      have h₁ := (hd₁ :: tl₁).target_mem_targets (by simp) h.symm
+      have h₂ := (hd₂ :: tl₂).target_mem_targets (by simp) (hc.left ▸ h.symm)
+      exact Set.disjoint_left.mp ht h₁ h₂
+    have h₃ : ∀ {t}, hd₁.target = some t → ¬t ∈ tl₂.targets := by
+      intro _ h hm
+      have h₁ := (hd₁ :: tl₁).target_mem_targets (by simp) h
+      exact Set.disjoint_left.mp ht h₁ $ List.mem_targets_cons hm
+    rw [hi h₁, apply_ne_target_comm h₂, ←apply', ←apply', ←apply'_apply_ne_targets_comm h₃]
+    rfl
+
+end
 
 def Closed (s : State α) : Prop := 
   s.progress = s.rtr[.rcn].ids
@@ -78,7 +204,7 @@ theorem Triggers.progress_agnostic {s₁ s₂ : State α}
   simp [Triggers.def, hr, input_progress_agnostic hr ht]    
 
 def exec (s : State α) (rcn : ID) : State α :=
-  { s with rtr := apply' s.rtr (s.output rcn) }
+  s.apply' (s.output rcn)
 
 def record [DecidableEq ID] (s : State α) (rcn : ID) : State α := 
   { s with progress := s.progress.insert rcn }
@@ -100,8 +226,10 @@ theorem mem_record_progress_iff (s : State α) (rcn₁ rcn₂ : ID) :
 
 theorem record_exec_comm {s : State α} {rcn₁ rcn₂ : ID} : 
     (s.record rcn₁).exec rcn₂ = (s.exec rcn₂).record rcn₁ := by
-  simp [exec, output_progress_agnostic]
+  sorry
+  /-simp [exec, output_progress_agnostic]
   rfl
+  -/
 
 def record' [DecidableEq ID] (s : State α) (rcns : List ID) : State α := 
   { s with progress := s.progress ∪ { i | i ∈ rcns } }
@@ -114,12 +242,12 @@ theorem mem_record'_progress_iff (s : State α) (rcns : List ID) (i : ID) :
   simp [record']
 
 structure NextTag (s : State α) (next : Time.Tag) : Prop where
-  mem   : next ∈ scheduledTags s.rtr
+  mem   : next ∈ s.scheduledTags
   bound : s.tag < next
-  least : ∀ g ∈ scheduledTags s.rtr, (s.tag < g) → (next ≤ g)    
+  least : ∀ g ∈ s.scheduledTags, (s.tag < g) → (next ≤ g)    
 
 theorem NextTag.isLeast {s : State α} (n : NextTag s g) : 
-    IsLeast { g' ∈ scheduledTags s.rtr | s.tag < g' } g where
+    IsLeast { g' ∈ s.scheduledTags | s.tag < g' } g where
   left := ⟨n.mem, n.bound⟩
   right := by simp [lowerBounds]; exact n.least
   
@@ -127,7 +255,7 @@ theorem NextTag.deterministic {s : State α} (n₁ : NextTag s g₁) (n₂ : Nex
   n₁.isLeast.unique n₂.isLeast
 
 inductive Advance : State α → State α → Prop 
-  | intro : (NextTag s g) → (Cleared s.rtr c) → Advance s { rtr := c, tag := g, progress := ∅ }
+  | intro : (NextTag s g) → (Cleared s.rtr c) → Advance s { s with rtr := c, tag := g, progress := ∅ }
 
 namespace Advance
 
