src/ReactorModel/Objects/Reactor/Updatable.lean
@@ -7,23 +7,23 @@ variable [ReactorType α]
 -- Note: Without ID-uniqueness this can be satisfied by updating exactly one of the occurrences of
 --       the target. Since we have a choice of which target we update, this type isn't a `Prop`. 
 --       (We need to be able to eliminate into `Type` in `Member.fromLawfulUpdate`).
-inductive LawfulMemUpdate (cpt : Component.Valued) (i : ID) (f : cpt.type → cpt.type) : α → α → Type
+inductive LawfulMemUpdate (cpt : Component.Valued) (i : ID) (v : Value) : α → α → Type
   | final : 
-    (rtr₁ ≃[cpt][i] rtr₂) → (rtr₁{cpt}{i} = some o) → (rtr₂{cpt}{i} = f o) → 
-    LawfulMemUpdate cpt i f rtr₁ rtr₂
+    (rtr₁ ≃[cpt][i] rtr₂) → (rtr₁{cpt}{i} = some o) → (rtr₂{cpt}{i} = v) → 
+    LawfulMemUpdate cpt i v rtr₁ rtr₂
   | nested : 
     (rtr₁ ≃[.rtr][j] rtr₂) → (rtr₁{.rtr}{j} = some n₁) → (rtr₂{.rtr}{j} = some n₂) → 
-    (LawfulMemUpdate cpt i f n₁ n₂) → LawfulMemUpdate cpt i f rtr₁ rtr₂
+    (LawfulMemUpdate cpt i v n₁ n₂) → LawfulMemUpdate cpt i v rtr₁ rtr₂
 
 -- Note: This isn't a `Prop` because of the explanation on `LawfulMemUpdate`.
-inductive LawfulUpdate (cpt : Component.Valued) (i : ID) (f : cpt.type → cpt.type) (rtr₁ rtr₂ : α)
-  | update (u : LawfulMemUpdate cpt i f rtr₁ rtr₂)
+inductive LawfulUpdate (cpt : Component.Valued) (i : ID) (v : Value) (rtr₁ rtr₂ : α)
+  | update (u : LawfulMemUpdate cpt i v rtr₁ rtr₂)
   | notMem (h : IsEmpty $ Member cpt i rtr₁) (eq : rtr₁ = rtr₂)
 
 class Updatable (α) extends ReactorType α where
-  update : α → (cpt : Component.Valued) → ID → (cpt.type → cpt.type) → α  
+  update : α → (cpt : Component.Valued) → ID → Value → α  
     
 class LawfulUpdatable (α) extends Updatable α where 
-  lawful : ∀ rtr cpt i f, LawfulUpdate cpt i f rtr (update rtr cpt i f)      
+  lawful : ∀ rtr cpt i v, LawfulUpdate cpt i v rtr (update rtr cpt i v)      
 
 end ReactorType
