src/ReactorModel/Objects/Component.lean
@@ -6,7 +6,6 @@ inductive Component.Valued
   | stv -- State variable
   | act -- Action
   
-
 -- An enumeration of the different *kinds* of components that are addressable by ids in a reactor.
 inductive Component
   | val (v : Component.Valued)
@@ -14,12 +13,6 @@ inductive Component
   | rcn -- Reactions
 
 namespace Component
-
-abbrev Valued.type : Valued → Type
-  | inp => Value
-  | out => Value
-  | stv => Value 
-  | act => Action
 
 @[match_pattern] abbrev inp := Component.val .inp
 @[match_pattern] abbrev out := Component.val .out
@@ -29,6 +22,7 @@ abbrev Valued.type : Valued → Type
 instance : Coe Component.Valued Component where
   coe := val 
 
+-- TODO: Can you replace all occurrences of this with just `WithTop ID`?
 -- The type of `WithTop ID`s extends the type of `ID`s with a `⊤` ID witch is used to refer to a/the
 -- top level reactor. We don't include the `⊤` ID in the normal `ID` type, as most contexts require
 -- that the `⊤` ID cannot not be used. For example, it should not be possible for a reaction to be
