src/ReactorModel/Objects/Reactor/Basic.lean
@@ -3,21 +3,12 @@ import ReactorModel.Objects.Reaction
 noncomputable section
 
 abbrev Component.type (rtrType : Type) : Component → Type
-  | .rtr     => rtrType 
-  | .rcn     => Reaction
-  | .val cpt => cpt.type
+  | .rtr   => rtrType 
+  | .rcn   => Reaction
+  | .val _ => Value
 
--- TODO: Generalize this over the `Component` type, so you can easily add things like connections.
---       In that case you whould have a type class for what constitutes a component type, which e.g.
---       would include requiring a mapping like `Reactor.Component.type` above.
---       How does this notion relate to the notion of functors?
---
--- Note: This approach is analogous to how algebras are defined in category theory, where the 
+-- Note: This approach is similar to how algebras are defined in category theory, where the 
 --       `Component` parameter plays the role of the functor over which the algrabra is defined.
---
--- TODO: Ask Andrès about how to proceed with this algebra based approach. E.g. if there are certain
---       kinds of mappings between algebras over different functors (which would correspond to 
---       reactor types over different kinds of components) which could be useful here.
 class ReactorType (α : Type) where
   get? : α → (cpt : Component) → (ID ⇀ cpt.type α)   
  
@@ -69,7 +60,6 @@ end Member
 inductive Object [ReactorType α] (rtr : α) (cpt : Component) (i : cpt.idType) : cpt.type α → Prop
   | intro (m : Member cpt i rtr) : Object rtr cpt i m.object
 
--- TODO: Find a better name for this.
 def RootEqualUpTo [ReactorType α] (cpt : Component) (i : ID) (rtr₁ rtr₂ : α) : Prop :=
   ∀ {c j}, (c ≠ cpt ∨ j ≠ i) → rtr₁{c}{j} = rtr₂{c}{j}
 
