src/ReactorModel/Objects/Reactor/Theorems/Accessible.lean
@@ -10,19 +10,19 @@ open Updatable Indexable
 
 variable [Accessible α] {rtr : α}
 
-theorem obj?_preserved (h : c ≠ cpt ∨ j ≠ i) : (update rtr cpt i f)[c][j] = rtr[c][j] :=
-  lawful rtr cpt i f |>.obj?_preserved h
+theorem obj?_preserved (h : c ≠ cpt ∨ j ≠ i) : (update rtr cpt i v)[c][j] = rtr[c][j] :=
+  lawful rtr cpt i v |>.obj?_preserved h
 
 theorem obj?_preserved_cpt (h : c ≠ cpt := by exact (nomatch ·)) : 
-    (update rtr cpt i f)[c][j] = rtr[c][j] :=
+    (update rtr cpt i v)[c][j] = rtr[c][j] :=
   obj?_preserved $ .inl h
 
 theorem obj?_preserved_id {c : Component.Valued} (h : j ≠ i) : 
-    (update rtr cpt i f)[c][j] = rtr[c][j] :=
+    (update rtr cpt i v)[c][j] = rtr[c][j] :=
   obj?_preserved $ .inr h
 
-theorem obj?_updated : (update rtr cpt i f)[cpt][i] = f <$> rtr[cpt][i] :=
-  lawful rtr cpt i f |>.obj?_updated
+theorem obj?_updated : (update rtr cpt i v)[cpt][i] = (fun _ => v) <$> rtr[cpt][i] :=
+  lawful rtr cpt i v |>.obj?_updated
 
 end LawfulUpdatable
 end ReactorType
