src/ReactorModel/Objects/Reactor/Theorems/Readable.lean
@@ -9,12 +9,11 @@ variable [Readable α] {rtr rtr₁ : α}
 
 -- TODO: For simplification of this proof, see comments above `StrictMember.rtr_equiv`.
 theorem LawfulMemUpdate.unique 
-    (u₁ : LawfulMemUpdate cpt i f rtr rtr₁) (u₂ : LawfulMemUpdate cpt i f rtr rtr₂) : 
+    (u₁ : LawfulMemUpdate cpt i v rtr rtr₁) (u₂ : LawfulMemUpdate cpt i v rtr rtr₂) : 
     rtr₁ = rtr₂ := by
   induction u₁ generalizing rtr₂ <;> cases u₂
-  case final.final e₁ h₁ h₁' _ h₂ h₂' e₂ =>
-    injection h₁ ▸ h₂ with h
-    exact RootEqualUpTo.ext (RootEqualUpTo.trans e₁.symm e₂) (h₂' ▸ h ▸ h₁')
+  case final.final e₁ _ h₁' _ _ h₂' e₂ =>
+    exact RootEqualUpTo.ext (RootEqualUpTo.trans e₁.symm e₂) (h₂' ▸ h₁')
   case nested.nested j₁ _ _ _ _ e₁ h₁ h₁' u₁ hi j₂ _ _ u₂ h₂ h₂' e₂ =>
     have h : j₁ = j₂ := by injection (u₁.member₁.nested h₁).unique (u₂.member₁.nested h₂)
     subst h; cases h₁ ▸ h₂; cases hi u₂
